WIP Call

Computation.v
@@ -5,17 +5,27 @@ Reserved Notation "x >>= y" (at level 42, right associativity).
 (*Reserved Notation "x <- y ; z" (at level 42, right associativity).
 Reserved Notation "x ;; z" (at level 42, right associativity).*)
 Reserved Notation "'call' f 'from' funcs [[ x ]]" (at level 35).
+Reserved Notation "'call' f [[ x ]]" (at level 35).
 
 Delimit Scope comp_scope with comp.
 Delimit Scope long_comp_scope with long_comp.
 
-Inductive Comp : Type -> Type :=
-| Return : forall A, A -> Comp A
-| Bind : forall A B, Comp A -> (A -> Comp B) -> Comp B
-| Pick : forall A, Ensemble A -> Comp A.
+Section Comp.
+  Variable names : Type.
+  Variables dom cod : names -> Type.
+
+  Inductive Comp : Type -> Type :=
+  | Return : forall A, A -> Comp A
+  | Bind : forall A B, Comp A -> (A -> Comp B) -> Comp B
+  | Pick : forall A, Ensemble A -> Comp A
+  | Call : forall name : names, Comp (dom name) -> Comp (cod name).
+End Comp.
 
 Bind Scope comp_scope with Comp.
-Arguments Bind A%type B%type _%comp _.
+Arguments Bind [_%type _ _ A%type B%type] _%comp _.
+Arguments Call [_%type _ _] name _%comp.
+Arguments Return [_ _ _ _] _.
+Arguments Pick [_ _ _ _] _.
 
 (*Notation "x >>= y" := (Bind x%comp y%comp) : comp_scope.
 Notation "x <- y ; z" := (Bind y%comp (fun x => z%comp)) : comp_scope.
@@ -31,15 +41,33 @@ Notation "x <- y ; z" := (Bind y%comp (fun x => z%comp))
 Notation "x ;; z" := (Bind x%comp (fun _ => z%comp))
                        (at level 81, right associativity,
                         format "'[v' x ;; '/' z ']'") : comp_scope.
-Notation "{ x  |  P }" := (@Pick _ (fun x => P)) : comp_scope.
-Notation "{ x : A  |  P }" := (@Pick A%type (fun x => P)) : comp_scope.
+Notation "{ x  |  P }" := (@Pick _ _ _ _ (fun x => P)) : comp_scope.
+Notation "{ x : A  |  P }" := (@Pick _ _ _ A%type (fun x => P)) : comp_scope.
+Notation "'call' f [[ x ]]" := (@Call _ _ _ f x) : comp_scope.
+
+Record BundledComp A :=
+  Bundle { CompNames : _;
+           CompDom : _;
+           CompCod : _;
+           Unbundle :> @Comp CompNames CompDom CompCod A;
+           Lookup : forall name, CompDom name -> @Comp CompNames CompDom CompCod (CompCod name)}.
+
+Delimit Scope bundled_comp_scope with bundled_comp.
+Bind Scope bundled_comp_scope with BundledComp.
+Open Scope bundled_comp_scope.
+
+Notation "``[ c 'with' l ]``" := (@Bundle _ _ _ _ c l) (only parsing) : bundled_comp_scope.
+Notation "`[ c ]`" := ``[ c with _ ]`` : bundled_comp_scope.
+Notation "``[ c 'with' l ]``" := (@Bundle _ _ _ _ c l) : long_comp_scope.
 
 Section comp.
-  Definition Lift A B (f : A -> B) : Comp A -> Comp B
+  Definition Lift names dom cod A B (f : A -> B)
+  : @Comp names dom cod A -> @Comp names dom cod B
     := fun x => (x' <- x;
                  Return (f x'))%comp.
 
-  Definition Or : Comp bool -> Comp bool -> Comp bool
+  Definition Or names dom cod
+  : @Comp names dom cod bool -> Comp _ _ bool -> Comp _ _ bool
     := fun c1 c2 =>
          (b1 <- c1;
           if b1
@@ -47,22 +75,34 @@ Section comp.
           else c2)%comp.
 
   Section computes_to.
-    Inductive computes_to
-    : forall A : Type, Comp A -> A -> Prop :=
+    Variable names : Type.
+    Variables dom cod : names -> Type.
+    Variable lookup : forall name, dom name -> @Comp names dom cod (cod name).
+
+    (** TODO(JasonGross): Should this be [CoInductive]? *)
+    Inductive computes_to : forall A, @Comp names dom cod A -> A -> Prop :=
     | ReturnComputes : forall A v, @computes_to A (Return v) v
     | BindComputes : forall A B comp_a f comp_a_value comp_b_value,
                        @computes_to A comp_a comp_a_value
                        -> @computes_to B (f comp_a_value) comp_b_value
                        -> @computes_to B (Bind comp_a f) comp_b_value
-    | PickComputes : forall A (P : Ensemble A) v, P v -> @computes_to A (Pick P) v.
+    | PickComputes : forall A (P : Ensemble A) v, P v -> @computes_to A (Pick P) v
+    | CallComputes : forall f x x_value fx_value,
+                       @computes_to (dom f) x x_value
+                       -> @computes_to (cod f) (@lookup f x_value) fx_value
+                       -> @computes_to _ (Call f x) fx_value.
 
-    Theorem computes_to_inv A (c : Comp A) v
-    : computes_to c v -> match c with
-                           | Return _ x => fun v => v = x
+    Theorem computes_to_inv A (c : @Comp names dom cod A) v
+    : computes_to c v -> match c in (@Comp _ _ _ A) return A -> Prop with
+                           | Return _ x => @eq _ x
                            | Bind _ _ x f => fun v => exists comp_a_value,
                                                         computes_to x comp_a_value
                                                         /\ computes_to (f comp_a_value) v
                            | Pick _ P => P
+                           | Call f x => fun fx_v =>
+                                           exists xv,
+                                             computes_to x xv
+                                             /\ computes_to (@lookup f xv) fx_v
                          end v.
     Proof.
       destruct 1; eauto.
@@ -76,7 +116,7 @@ Section comp.
         forall v, computes_to c v -> P v.
 
       (* Relation to assist in building proofs of compuational_inv *)
-      Inductive CompInv : forall {A : Type}, Ensemble A -> Comp A -> Prop :=
+      Inductive CompInv : forall {A : Type}, Ensemble A -> @Comp names dom cod A -> Prop :=
       | Return_Inv : forall A (a : A) (P : Ensemble A),
                        P a -> CompInv P (Return a)
       | Bind_Inv : forall A B (PA : Ensemble A) (PB : Ensemble B) comp_a comp_f,
@@ -84,15 +124,22 @@ Section comp.
                      (forall (a : A), PA a -> CompInv PB (comp_f a)) ->
                      CompInv PB (Bind comp_a comp_f)
       | Pick_Inv : forall A (P P' : Ensemble A),
-                     (forall a, P a -> P' a) -> CompInv P' (Pick P).
+                     (forall a, P a -> P' a) -> CompInv P' (Pick P)
+      | Call_Inv : forall f P P' comp_x,
+                       @CompInv (dom f) P comp_x
+                       -> (forall x, P x -> CompInv P' (@lookup f x))
+                       -> CompInv P' (Call f comp_x).
 
       Lemma CompInv_inv A c (P : Ensemble A)
-      : CompInv P c -> match c with
+      : CompInv P c -> match c in (@Comp _ _ _ A) return Ensemble A -> Prop with
                          | Return A x => fun P => P x
                          | Bind A B x f => fun PB => exists PA : Ensemble A,
                                                        CompInv PA x /\
                                                        forall b : A, PA b -> CompInv PB (f b)
                          | Pick A P => fun P' => (forall a, P a -> P' a)
+                         | Call f x => fun P' => exists P,
+                                                   CompInv P x
+                                                   /\ forall xv, P xv -> CompInv P' (@lookup f xv)
                        end P.
       Proof.
         destruct 1; eauto.
@@ -103,45 +150,59 @@ Section comp.
       Lemma CompInv_compuational_inv A (P : Ensemble A) c
       : CompInv P c -> computational_inv P c.
       Proof.
-        induction c; intros; apply_in_hyp_no_cbv_match CompInv_inv; simpl;
-        intros; apply_in_hyp_no_cbv_match computes_to_inv; subst; eauto.
-        destruct_ex; split_and; simpl in *;
-        eapply H; eauto; eapply H4; eapply IHc; eauto.
+        induction c;
+        intros; inversion_by CompInv_inv; simpl in *;
+        intros; inversion_by computes_to_inv; simpl in *; subst;
+        destruct_ex; split_and;
+        eauto;
+        try solve [ specialize_all_ways; eauto ].
+        admit.
       Qed.
-
-  End CompInv.
-
+    End CompInv.
   End computes_to.
 
   Section is_computational.
-    (** A [Comp] is maximally computational if it could be written without [Pick] *)
-    Inductive is_computational : forall A, Comp A -> Prop :=
+    Variable names : Type.
+    Variables dom cod : names -> Type.
+    Variable lookup : forall name, dom name -> @Comp names dom cod (cod name).
+
+    (** A [Comp] is maximally computational if it could be written without [Pick].  For now, we don't permit [Call] in computational things, because the halting problem. *)
+    Inductive is_computational : forall A, @Comp names dom cod A -> Prop :=
     | Return_is_computational : forall A (x : A), is_computational (Return x)
-    | Bind_is_computational : forall A B (cA : Comp A) (f : A -> Comp B),
+    | Bind_is_computational : forall A B (cA : Comp _ _ A) (f : A -> Comp _ _ B),
                                 is_computational cA
                                 -> (forall a,
-                                      computes_to cA a -> is_computational (f a))
-                                -> is_computational (Bind cA f).
+                                      @computes_to names dom cod lookup _ cA a -> is_computational (f a))
+                                -> is_computational (Bind cA f)
+(*    | Call_is_computational : forall f x,
+                                is_computational x
+                                -> (forall xv,
+                                      @computes_to names dom cod lookup _ x xv
+                                      -> is_computational (@lookup f xv))
+                                -> is_computational (Call f x)*).
 
-    Theorem is_computational_inv A (c : Comp A)
+    Theorem is_computational_inv A (c : @Comp names dom cod A)
     : is_computational c
       -> match c with
            | Return _ _ => True
            | Bind _ _ x f => is_computational x
-                             /\ forall v, computes_to x v
+                             /\ forall v, @computes_to names dom cod lookup _ x v
                                           -> is_computational (f v)
            | Pick _ _ => False
+           | Call f x => False (*is_computational x
+                         /\ forall v, @computes_to names dom cod lookup _ x v
+                                      -> is_computational (@lookup f v)*)
          end.
     Proof.
       destruct 1; eauto.
     Qed.
 
     (** It's possible to extract the value from a fully detiministic computation *)
-    Fixpoint is_computational_unique_val A (c : Comp A)
-    : is_computational c -> { a | unique (computes_to c) a }.
+    Fixpoint is_computational_unique_val A (c : @Comp names dom cod A) {struct c}
+    : is_computational c -> { a | unique (computes_to lookup c) a }.
     Proof.
-      refine match c as c return is_computational c -> { a | unique (computes_to c) a } with
-               | Return T x => fun _ => existT (unique (computes_to (ret x)))
+      refine match c as c return is_computational c -> { a | unique (computes_to lookup c) a } with
+               | Return T x => fun _ => existT (unique (computes_to lookup (ret x)))
                                                x
                                                _
                | Pick _ _ => fun H => match is_computational_inv H with end
@@ -150,36 +211,43 @@ Section comp.
                     => let H' := is_computational_inv H in
                        let xv := @is_computational_unique_val _ _ (proj1 H') in
                        let fxv := @is_computational_unique_val _ _ (proj2 H' _ (proj1 (proj2_sig xv))) in
-                       exist (unique (computes_to _))
+                       exist (unique (computes_to _ _))
                              (proj1_sig fxv)
                              _
+               | Call f x => fun H => match is_computational_inv H with end(*
+                               let H' := is_computational_inv H in
+                               let xv := @is_computational_unique_val _ _ (proj1 H') in
+                               let fxv := @is_computational_unique_val _ _ (proj2 H' _ (proj1 (proj2_sig xv))) in
+                               exist (unique (computes_to _ _))
+                                     (proj1_sig fxv)
+                                     _*)
              end;
       clearbodies;
       clear is_computational_unique_val;
-      [ abstract (repeat econstructor; intros; inversion_by computes_to_inv; eauto)
-      | abstract (
-            simpl in *;
-            unfold unique in *;
-            destruct_sig;
-            repeat econstructor;
-            intros;
-            eauto;
-            inversion_by computes_to_inv;
-            apply_hyp;
-            do_with_hyp ltac:(fun H => erewrite H by eassumption);
-            eassumption
-          ) ].
+      first [ abstract (repeat econstructor; intros; inversion_by computes_to_inv; eauto)
+            | abstract (
+                  simpl in *;
+                  unfold unique in *;
+                  destruct_sig;
+                  repeat econstructor;
+                  intros;
+                  eauto;
+                  inversion_by computes_to_inv;
+                  apply_hyp;
+                  do_with_hyp ltac:(fun H => erewrite H by eassumption);
+                  eassumption
+                ) ].
     Defined.
 
-    Definition is_computational_val A (c : Comp A) (H : is_computational c) : A
+    Definition is_computational_val A (c : @Comp names dom cod A) (H : is_computational c) : A
       := proj1_sig (@is_computational_unique_val A c H).
-    Definition is_computational_val_computes_to A (c : Comp A) (H : is_computational c) : computes_to c (is_computational_val H)
+    Definition is_computational_val_computes_to A (c : @Comp names dom cod A) (H : is_computational c) : computes_to lookup c (is_computational_val H)
       := proj1 (proj2_sig (@is_computational_unique_val A c H)).
-    Definition is_computational_val_unique A (c : Comp A) (H : is_computational c)
-    : forall x, computes_to c x -> is_computational_val H = x
+    Definition is_computational_val_unique A (c : @Comp names dom cod A) (H : is_computational c)
+    : forall x, computes_to lookup c x -> is_computational_val H = x
       := proj2 (proj2_sig (@is_computational_unique_val A c H)).
-    Definition is_computational_val_all_eq A (c : Comp A) (H : is_computational c)
-    : forall x y, computes_to c x -> computes_to c y -> x = y.
+    Definition is_computational_val_all_eq A (c : @Comp names dom cod A) (H : is_computational c)
+    : forall x y, computes_to lookup c x -> computes_to lookup c y -> x = y.
     Proof.
       intros.
       transitivity (@is_computational_val A c H); [ symmetry | ];
@@ -189,6 +257,10 @@ Section comp.
   End is_computational.
 
   Section monad.
+    Variable names : Type.
+    Variables dom cod : names -> Type.
+    Variable lookup : forall name, dom name -> @Comp names dom cod (cod name).
+
     Local Ltac t :=
       split;
       intro;
@@ -203,30 +275,30 @@ Section comp.
                    | solve [ constructor ]
                    | eapply BindComputes; (eassumption || (try eassumption; [])) ].
 
-    Lemma bind_bind X Y Z (f : X -> Comp Y) (g : Y -> Comp Z) x v
-    : computes_to (Bind (Bind x f) g) v
-      <-> computes_to (Bind x (fun u => Bind (f u) g)) v.
+    Lemma bind_bind X Y Z (f : X -> @Comp names dom cod Y) (g : Y -> @Comp _ _ _ Z) x v
+    : computes_to lookup (Bind (Bind x f) g) v
+      <-> computes_to lookup (Bind x (fun u => Bind (f u) g)) v.
     Proof.
       t.
     Qed.
 
-    Lemma bind_unit X Y (f : X -> Comp Y) x v
-    : computes_to (Bind (Return x) f) v
-      <-> computes_to (f x) v.
+    Lemma bind_unit X Y (f : X -> @Comp names dom cod Y) x v
+    : computes_to lookup (Bind (Return x) f) v
+      <-> computes_to lookup (f x) v.
     Proof.
       t.
     Qed.
 
-    Lemma unit_bind X (x : Comp X) v
-    : computes_to (Bind x (@Return X)) v
-      <-> computes_to x v.
+    Lemma unit_bind X (x : @Comp names dom cod X) v
+    : computes_to lookup (Bind x (@Return _ _ _ X)) v
+      <-> computes_to lookup x v.
     Proof.
       t.
     Qed.
 
-    Lemma computes_under_bind X Y (f g : X -> Comp Y) x
-    : (forall x v, computes_to (f x) v <-> computes_to (g x) v) ->
-      (forall v, computes_to (Bind x f) v <-> computes_to (Bind x g) v).
+    Lemma computes_under_bind X Y (f g : X -> @Comp names dom cod Y) x
+    : (forall x v, computes_to lookup (f x) v <-> computes_to lookup (g x) v) ->
+      (forall v, computes_to lookup (Bind x f) v <-> computes_to lookup (Bind x g) v).
     Proof.
       t; split_iff; eauto.
     Qed.
@@ -236,56 +308,97 @@ Section comp.
   (** The old program might be non-deterministic, and the new program
       less so.  This means we want to say that if [new] can compute to
       [v], then [old] should be able to compute to [v], too. *)
-  Definition refine {A} (old new : Comp A)
-    := forall v, computes_to new v -> computes_to old v.
+  Definition refine {A} {oldNames oldDom oldCod newNames newDom newCod}
+             oldLookup newLookup
+             (old : @Comp oldNames oldDom oldCod A)
+             (new : @Comp newNames newDom newCod A)
+    := forall v, computes_to newLookup new v -> computes_to oldLookup old v.
+  Definition refineBundled {A} (old new : BundledComp A)
+    := refine (Lookup old) (Lookup new) old new.
+
+  Global Arguments refineBundled : simpl never.
+  Typeclasses Transparent refineBundled.
 
   (** Define a symmetrized version of [refine] for ease of rewriting *)
-  Definition refineEquiv {A} (old new : Comp A)
-    := refine old new /\ refine new old.
+  Definition refineEquiv {A} {oldNames oldDom oldCod newNames newDom newCod}
+             oldLookup newLookup
+             (old : @Comp oldNames oldDom oldCod A)
+             (new : @Comp newNames newDom newCod A)
+    := refine oldLookup newLookup old new /\ refine newLookup oldLookup new old.
 
-  Global Instance refine_PreOrder A
-  : PreOrder (@refine A).
-  Proof.
-    split; compute in *; eauto.
-  Qed.
+  Definition refineBundledEquiv {A} (old new : BundledComp A)
+    := refineEquiv (Lookup old) (Lookup new) old new.
 
-  Global Instance refineEquiv_Equivalence A
-  : Equivalence (@refineEquiv A).
-  Proof.
-    repeat (split || intro); compute in *; split_and; eauto.
-  Qed.
+  Global Arguments refineBundledEquiv : simpl never.
+  Typeclasses Transparent refineBundledEquiv.
+
+  Local Obligation Tactic := repeat first [ solve [ eauto ]
+                                          | progress hnf in *
+                                          | intro
+                                          | split
+                                          | progress split_and ].
+
+  Global Program Instance refine_PreOrder A names dom cod lookup : PreOrder (@refine A names dom cod names dom cod lookup lookup).
+  Global Program Instance refineBundled_PreOrder A : PreOrder (@refineBundled A).
+  Global Program Instance refineEquiv_Equivalence A names dom cod lookup : Equivalence (@refineEquiv A names dom cod names dom cod lookup lookup).
+  Global Program Instance refineBundledEquiv_Equivalence A : Equivalence (@refineBundledEquiv A).
 
   Section monad_refine.
-    Lemma refineEquiv_bind_bind X Y Z (f : X -> Comp Y) (g : Y -> Comp Z) x
-    : refineEquiv (Bind (Bind x f) g)
+    Variable names : Type.
+    Variables dom cod : names -> Type.
+    Variable lookup : forall name, dom name -> @Comp names dom cod (cod name).
+
+    Lemma refineEquiv_bind_bind X Y Z (f : X -> @Comp names dom cod Y) (g : Y -> @Comp _ _ _ Z) x
+    : refineEquiv lookup lookup
+                  (Bind (Bind x f) g)
                   (Bind x (fun u => Bind (f u) g)).
     Proof.
       split; intro; apply bind_bind.
     Qed.
 
-    Lemma refineEquiv_bind_unit X Y (f : X -> Comp Y) x
-    : refineEquiv (Bind (Return x) f)
+    Definition refineBundledEquiv_bind_bind
+    : forall X Y Z f g x, refineBundledEquiv ``[ _ with lookup ]`` ``[ _ with lookup ]``
+      := refineEquiv_bind_bind.
+
+    Lemma refineEquiv_bind_unit X Y (f : X -> @Comp names dom cod Y) x
+    : refineEquiv lookup lookup
+                  (Bind (Return x) f)
                   (f x).
     Proof.
-      split; intro; apply bind_unit.
+      split; intro; simpl; apply bind_unit.
     Qed.
 
-    Lemma refineEquiv_unit_bind X (x : Comp X)
-    : refineEquiv (Bind x (@Return X))
+    Definition refineBundledEquiv_bind_unit
+    : forall X Y f x, refineBundledEquiv ``[ _ with lookup ]`` ``[ _ with lookup ]``
+      := refineEquiv_bind_unit.
+
+    Lemma refineEquiv_unit_bind X (x : @Comp _ _ _ X)
+    : refineEquiv lookup lookup
+                  (Bind x (@Return _ _ _ X))
                   x.
     Proof.
       split; intro; apply unit_bind.
     Qed.
 
-    Lemma refineEquiv_under_bind X Y (f g : X -> Comp Y) x
-          (eqv_f_g : forall x, refineEquiv (f x) (g x))
-    : refineEquiv (Bind x f)
-                  (Bind x g).
-      Proof.
-        split; unfold refine; intros; eapply computes_under_bind;
-        eauto; split; eapply eqv_f_g.
-      Qed.
+    Definition refineBundledEquiv_unit_bind
+    : forall X x, refineBundledEquiv ``[ _ with lookup ]`` ``[ _ with lookup ]``
+      := refineEquiv_unit_bind.
 
+    Lemma refineEquiv_under_bind X Y (f g : X -> @Comp _ _ _ Y) x
+          (eqv_f_g : forall x, refineEquiv lookup lookup (f x) (g x))
+    : refineEquiv lookup lookup
+                  (Bind x f)
+                  (Bind x g).
+    Proof.
+      split; unfold refine; simpl in *; intros; eapply computes_under_bind;
+      intros; eauto; split; eapply eqv_f_g.
+    Qed.
+
+    Definition refineBundledEquiv_under_bind
+    : forall X Y f g x
+             (equv_f_g : forall x, refineBundledEquiv ``[ _ with lookup ]`` ``[ _ with lookup ]``),
+        refineBundledEquiv ``[ _ with lookup ]`` ``[ _ with lookup ]``
+      := refineEquiv_under_bind.
   End monad_refine.
 End comp.
 
@@ -294,183 +407,270 @@ Ltac inversion_by rule :=
                         | progress split_and
                         | apply_in_hyp_no_cbv_match rule ].
 
-Add Parametric Relation A : (Comp A) (@refine A)
+Add Parametric Relation A names dom cod lookup
+: (@Comp names dom cod A) (@refine A names dom cod names dom cod lookup lookup)
   reflexivity proved by reflexivity
   transitivity proved by transitivity
     as refine_rel.
 
-Add Parametric Relation A : (Comp A) (@refineEquiv A)
+Add Parametric Relation A
+: (BundledComp A) (@refineBundled A)
+  reflexivity proved by reflexivity
+  transitivity proved by transitivity
+    as refineBundled_rel.
+
+Add Parametric Relation A names dom cod lookup
+: (@Comp names dom cod A) (@refineEquiv A names dom cod names dom cod lookup lookup)
   reflexivity proved by reflexivity
   symmetry proved by symmetry
   transitivity proved by transitivity
     as refineEquiv_rel.
 
-Add Parametric Morphism A : (@refine A)
+Add Parametric Relation A
+: (BundledComp A) (@refineBundledEquiv A)
+  reflexivity proved by reflexivity
+  symmetry proved by symmetry
+  transitivity proved by transitivity
+    as refineBundledEquiv_rel.
+
+Local Ltac t := unfold impl; intros; repeat (eapply_hyp || etransitivity).
+
+Add Parametric Morphism A names dom cod lookup
+: (@refine A names dom cod names dom cod lookup lookup)
   with signature
-  (@refineEquiv A) --> (@refineEquiv A) ++> impl
+  (@refine A names dom cod names dom cod lookup lookup) --> (@refine A names dom cod names dom cod lookup lookup) ++> impl
     as refine_refine.
-Proof.
-  unfold impl.
-  intros.
-  repeat (eapply_hyp || etransitivity).
-Qed.
+Proof. t. Qed.
+
+(*Add Parametric Morphism A names dom cod lookup
+: (@refine A names dom cod names dom cod lookup lookup)
+  with signature
+  (@refineEquiv A names dom cod names dom cod lookup lookup) --> (@refineEquiv A names dom cod names dom cod lookup lookup) ++> impl
+    as refine_refineEquiv.
+Proof. t. Qed.*)
+
+
+Add Parametric Morphism A
+: (@refineBundled A)
+  with signature
+  (@refineBundled A) --> (@refineBundled A) ++> impl
+    as refineBundled_refineBundled.
+Proof. t. Qed.
+
+(*Add Parametric Morphism A
+: (@refineBundled A)
+  with signature
+  (@refineBundledEquiv A) --> (@refineBundledEquiv A) ++> impl
+    as refineBundled_refineBundledEquiv.
+Proof. t. Qed.*)
 
 Hint Constructors CompInv computes_to.
 
-Add Parametric Morphism A B : (@Bind A B)
-  with signature
-  (@refine A)
-    ==> (pointwise_relation _ (@refine B))
-    ==> (@refine B)
-    as refine_bind.
+Add Parametric Morphism names dom cod lookup A B
+: (@Bind names dom cod A B)
+    with signature
+    (@refine A names dom cod names dom cod lookup lookup)
+      ==> (pointwise_relation _ (@refine B names dom cod names dom cod lookup lookup))
+      ==> (@refine B names dom cod names dom cod lookup lookup)
+      as refine_bind.
 Proof.
-  intros.
-  unfold pointwise_relation, refine in *.
+  simpl; intros.
+  unfold pointwise_relation, refine in *; simpl in *.
   intros.
   inversion_by computes_to_inv.
   eauto.
 Qed.
 
-Add Parametric Morphism A B : (@Bind A B)
-  with signature
-  (@refineEquiv A)
-    ==> (pointwise_relation _ (@refineEquiv B))
-    ==> (@refineEquiv B)
-    as refineEquiv_bind.
+Add Parametric Morphism names dom cod lookup A B
+: (@Bind names dom cod A B)
+    with signature
+    (@refineEquiv A names dom cod names dom cod lookup lookup)
+      ==> (pointwise_relation _ (@refineEquiv B names dom cod names dom cod lookup lookup))
+      ==> (@refineEquiv B names dom cod names dom cod lookup lookup)
+      as refineEquiv_bind.
 Proof.
-  intros.
+  simpl; intros.
   unfold pointwise_relation, refineEquiv, refine in *.
-  split_and.
+  split_and; simpl in *.
   split; intros;
   inversion_by computes_to_inv;
   eauto.
 Qed.
 
-Add Parametric Morphism A B : (@Bind A B)
-  with signature
-  (@refineEquiv A)
-    ==> (pointwise_relation _ (@refineEquiv B))
-    ==> (@refine B)
-    as refineEquiv_refine_bind.
+(*Add Parametric Morphism names dom cod lookup A B
+: (@Bind names dom cod A B)
+    with signature
+    (@refineEquiv A names dom cod names dom cod lookup lookup)
+      ==> (pointwise_relation _ (@refineEquiv B names dom cod names dom cod lookup lookup))
+      ==> (@refine B names dom cod names dom cod lookup lookup)
+      as refineEquiv_refine_bind.
 Proof.
   intros.
-  refine (proj1 (_ : refineEquiv _ _)).
+  refine (proj1 (_ : refineEquiv _ _ _ _)).
+  simpl in *.
+  setoid_rewrite <- H.
   setoid_rewrite_hyp.
   reflexivity.
-Qed.
+Qed.*)
 
-Arguments impl _ _ / .
-Arguments computational_inv A P c / .
+Local Arguments impl _ _ / .
+Global Arguments computational_inv [names dom cod] lookup [A] P c / .
 
-Add Parametric Morphism A P : (@computational_inv A P)
+Add Parametric Morphism names dom cod lookup A P : (@computational_inv names dom cod lookup A P)
   with signature
-  (@refine A) ++> impl
+  (@refine A names dom cod names dom cod lookup lookup) ++> impl
     as refineCompInv.
-Proof.
-  simpl; eauto.
-Qed.
+Proof. simpl; eauto. Qed.
 
 Section general_refine_lemmas.
+  Local Ltac t :=
+    repeat first [ progress eauto
+                 | eassumption
+                 | progress split_iff
+                 | progress inversion_by computes_to_inv
+                 | progress subst
+                 | intro
+                 | econstructor
+                 | erewrite is_computational_val_unique
+                 | progress destruct_head_hnf prod
+                 | progress destruct_head_hnf and
+                 | progress specialize_all_ways ].
 
-  Lemma refineEquiv_is_computational A (c : Comp A) (CompC : is_computational c)
-  : refineEquiv c (ret (is_computational_val CompC)).
+  Lemma refineEquiv_is_computational A {names dom cod names' dom' cod'} (c : @Comp names dom cod A) lookup lookup' (CompC : is_computational lookup c)
+  : @refineEquiv _ names dom cod names' dom' cod' lookup lookup'
+                c (ret (is_computational_val CompC)).
   Proof.
     unfold refineEquiv, refine.
     pose proof (is_computational_val_computes_to CompC).
-    repeat (intro || split);
-    try inversion_by computes_to_inv; subst; trivial.
-    erewrite is_computational_val_unique; eauto.
+    t.
   Qed.
 
-  Lemma refine_pick A (P : A -> Prop) c (H : forall x, computes_to c x -> P x)
-  : refine { x : A | P x }%comp
-           c.
-  Proof.
-    repeat intro;
-    specialize_all_ways;
-    econstructor;
-    trivial.
-  Defined.
+  Definition refineBundledEquiv_is_computational A {names dom cod} (c : BundledComp A) lookup
+  : forall (CompC : is_computational (Lookup c) c),
+      refineBundledEquiv c (@Bundle A names dom cod (ret (is_computational_val CompC)) lookup)
+    := refineEquiv_is_computational lookup.
 
-  Lemma refine_pick_pick A (P1 P2 : A -> Prop)
+  Lemma refine_pick A {names dom cod names' dom' cod'} lookup lookup'
+        (P : A -> Prop) c (H : forall x, computes_to lookup' c x -> P x)
+  : @refine A names dom cod names' dom' cod' lookup lookup'
+            { x : A | P x }%comp
+            c.
+  Proof. t. Qed.
+
+  Definition refineBundled_pick A {names dom cod} lookup
+             P (c : BundledComp A)
+  : _ -> refineBundled ``[ { x : A | P x }%comp with lookup ]``
+                       c
+    := @refine_pick _ names dom cod _ _ _ lookup _ P c.
+
+  Lemma refine_pick_pick A {names dom cod names' dom' cod'} lookup lookup' (P1 P2 : A -> Prop)
         (H : forall x, P2 x -> P1 x)
-  : refine { x : A | P1 x }%comp
-           { x : A | P2 x }%comp.
-  Proof.
-    apply refine_pick;
-    intros;
-    inversion_by computes_to_inv;
-    auto.
-  Defined.
+  : @refine _ names dom cod names' dom' cod' lookup lookup'
+            { x : A | P1 x }%comp
+            { x : A | P2 x }%comp.
+  Proof. t. Qed.
 
-  Lemma refineEquiv_pick_pick A (P1 P2 : A -> Prop)
+  Definition refineBundled_pick_pick
+  : forall A {names dom cod names' dom' cod'} lookup lookup' P1 P2 H,
+      refineBundled ``[ _ with lookup ]``
+                    ``[ _ with lookup' ]``
+    := refine_pick_pick.
+
+  Lemma refineEquiv_pick_pick A {names dom cod names' dom' cod'} lookup lookup' (P1 P2 : A -> Prop)
         (H : forall x, P1 x <-> P2 x)
-  : refineEquiv { x : A | P1 x }%comp
-                { x : A | P2 x }%comp.
-  Proof.
-    split_iff.
-    split;
-    apply refine_pick_pick;
-    assumption.
-  Defined.
+  : @refineEquiv _ names dom cod names' dom' cod' lookup lookup'
+                 { x : A | P1 x }%comp
+                 { x : A | P2 x }%comp.
+  Proof. t. Qed.
 
-  Lemma refine_pick_pair A B (PA : A -> Prop) (PB : B -> Prop)
-  : refine { x : A * B | PA (fst x) /\ PB (snd x) }%comp
-           (a <- { a : A | PA a };
-            b <- { b : B | PB b };
-            ret (a, b))%comp.
-  Proof.
-    apply refine_pick.
-    intro x.
-    repeat constructor;
-    inversion_by computes_to_inv; subst; trivial.
-  Qed.
+  Definition refineBundledEquiv_pick_pick
+  : forall A {names dom cod names' dom' cod'} lookup lookup' P1 P2 H,
+      refineBundledEquiv ``[ _ with lookup ]``
+                         ``[ _ with lookup' ]``
+    := refineEquiv_pick_pick.
 
+  Lemma refineEquiv_pick_pair {names dom cod names' dom' cod'} lookup lookup' A B (PA : A -> Prop) (PB : B -> Prop)
+  : @refineEquiv _ names dom cod names' dom' cod' lookup lookup'
+                 { x : A * B | PA (fst x) /\ PB (snd x) }%comp
+                 (a <- { a : A | PA a };
+                  b <- { b : B | PB b };
+                  ret (a, b))%comp.
+  Proof. t. Qed.
 
-  Definition refineEquiv_split_ex A B (P : A -> Prop) (P' : A -> B -> Prop)
-  : refineEquiv { b | exists a, P a /\ P' a b }%comp
-                (a <- { a | P a /\ exists b, P' a b };
-                 { b | P' a b })%comp.
-  Proof.
-    split;
-    hnf; intros;
-    inversion_by computes_to_inv;
-    repeat econstructor;
-    eassumption.
-  Qed.
+  Definition refineEquivBundled_pick_pair
+  : forall A {names dom cod names' dom' cod'} lookup lookup' P1 P2 H,
+      refineBundledEquiv ``[ _ with lookup ]``
+                         ``[ _ with lookup' ]``
+    := refineEquiv_pick_pick.
 
-  Definition refineEquiv_pick_contr_ret A (P : A -> Prop)
+  Definition refineEquiv_split_ex {names dom cod names' dom' cod'} lookup lookup' A B (P : A -> Prop) (P' : A -> B -> Prop)
+  : @refineEquiv _ names dom cod names' dom' cod' lookup lookup'
+                 { b | exists a, P a /\ P' a b }%comp
+                 (a <- { a | P a /\ exists b, P' a b };
+                  { b | P' a b })%comp.
+  Proof. t. Qed.
+
+  Definition refineBundledEquiv_split_ex
+  : forall {names dom cod names' dom' cod'} lookup lookup' A B P P',
+      refineBundledEquiv `[ _ ]` `[ _ ]`
+    := @refineEquiv_split_ex.
+
+  Definition refineEquiv_pick_contr_ret {names dom cod names' dom' cod'} lookup lookup' A (P : A -> Prop)
              (x : A) (H : unique P x)
-  : refineEquiv { y | P y }
-                (ret x).
+  : @refineEquiv _ names dom cod names' dom' cod' lookup lookup'
+                 { y | P y }
+                 (ret x).
+  Proof. t. Qed.
+
+  Definition refineEquiv_pick_eq {names dom cod names' dom' cod'} lookup lookup'
+             A (x : A)
+  : @refineEquiv _ names dom cod names' dom' cod' lookup lookup'
+                 { y | y = x }%comp
+                 (ret x).
+  Proof. t. Qed.
+
+  Definition refineBundledEquiv_pick_eq
+  : forall {names dom cod names' dom' cod'} lookup lookup'
+           A (x : A),
+      refineBundledEquiv `[ _ ]` `[ _ ]`
+    := @refineEquiv_pick_eq.
+
+  Definition refineEquiv_pick_eq' {names dom cod names' dom' cod'} lookup lookup'
+             A (x : A)
+  : @refineEquiv _ names dom cod names' dom' cod' lookup lookup'
+                 { y | x = y }%comp
+                 (ret x).
+  Proof. t. Qed.
+
+  Definition refineBundledEquiv_pick_eq'
+  : forall {names dom cod names' dom' cod'} lookup lookup'
+           A (x : A),
+      refineBundledEquiv `[ _ ]` `[ _ ]`
+    := @refineEquiv_pick_eq'.
+
+  Definition refineBundledEquiv_split_func_ex {names dom cod names' dom' cod'} lookup lookup'
+             A B (P : A -> Prop) (f : A -> B)
+  : refineBundledEquiv (@Bundle _ names dom cod { b | exists a, P a /\ b = f a}%comp lookup)
+                       (@Bundle _ names' dom' cod'
+                                (a <- { a | P a};
+                                 ret (f a))%comp
+                                lookup').
   Proof.
-    split; hnf; intros;
-    inversion_by computes_to_inv;
-    destruct_head_hnf and;
-    specialize_all_ways; subst;
-    econstructor; assumption.
+    repeat setoid_rewrite refineBundledEquiv_split_ex.
+    (** I want to just [setoid_rewrite refineBundledEquiv_pick_eq].  But I can't because things don't line up nicely, and there are no parameterized setoid relations.  :-( *)
+    erewrite refineEquiv_pick_pick.
+    - reflexivity.
+    - abstract (repeat (intro || esplit); intuition).
   Qed.
 
-  Definition refineEquiv_pick_eq A (x : A)
-  : refineEquiv { y | y = x }%comp
-                (ret x).
+  Definition refineEquiv_split_func_ex {names dom cod names' dom' cod'} lookup lookup'
+             A B (P : A -> Prop) (f : A -> B)
+  : @refineEquiv _ names dom cod names' dom' cod' lookup lookup'
+                 { b | exists a, P a /\ b = f a}%comp
+                 (a <- { a | P a};
+                  ret (f a))%comp.
   Proof.
-    apply refineEquiv_pick_contr_ret; firstorder.
-  Qed.
-
-  Definition refineEquiv_pick_eq' A (x : A)
-  : refineEquiv { y | x = y }%comp
-                (ret x).
-  Proof.
-    apply refineEquiv_pick_contr_ret; firstorder.
-  Qed.
-
-  Definition refineEquiv_split_func_ex A B (P : A -> Prop) (f : A -> B)
-  : refineEquiv { b | exists a, P a /\ b = f a}%comp
-                (a <- { a | P a};
-                 ret (f a))%comp.
-  Proof.
-    repeat setoid_rewrite refineEquiv_split_ex.
+    repeat setoid_rewrite refineBundledEquiv_split_ex.
     setoid_rewrite refineEquiv_pick_eq.
     erewrite refineEquiv_pick_pick.
     - reflexivity.
